spec only version

CheriInstSpec.v
@@ -1,511 +1,1100 @@
-Require Import Kami.AllNotations ProcKami.CheriTypes.
+Require Import Kami.AllNotations ProcKami.CheriTypes ProcKami.Lib.
 Require Import List.
 
-Section InstSpec.
+Section InstBaseSpec.
   Context `{procParams: ProcParams}.
   Local Open Scope kami_expr.
 
-  Definition SpecOutput :=
+  Definition BaseOutput :=
     STRUCT_TYPE {
         "wb?" :: Bool;
         "cdTag" :: Bool;
         "cdCap" :: Cap;
         "cdVal" :: Data;
+        "mayChangePc?" :: Bool;
         "taken?" :: Bool;
-        "takenPc" :: Addr;
-        "takenPcCapChange?" :: Bool;
-        "takenPcCap" :: Cap;
+        "pcMemAddr" :: Addr;
+        "changePcCap?" :: Bool;
+        "pcCap" :: Cap;
+        "changeIe?" :: Bool;
+        "newIe" :: Bool;
         "exception?" :: Bool;
         "exceptionCause" :: Data;
-        "memAddr" :: Addr;
+        "exceptionCausePc?" :: Bool;
+        "mem?" :: Bool;
         "memCap?" :: Bool;
         "memSize" :: MemSize;
-        "load?" :: Bool;
-        "ldSigned?" :: Bool;
-        "ldLG" :: Bool;
-        "ldLM" :: Bool;
-        "ldMC" :: Bool;
         "store?" :: Bool;
-        "stData" :: FullCapWithTag }.
+        "ldSigned?" :: Bool;
+        "ldPerms" :: CapPerms;
+        "interrupt?" :: Bool }.
 
   Section ty.
     Variable ty: Kind -> Type.
-    Definition DefSpecOutput: SpecOutput @# ty :=
-      (Const _ (getDefaultConst _)).
+    Definition DefBaseOutput: BaseOutput @# ty := Const _ Default.
 
-    Definition Trunc32Signed m n (e: Bit n @# ty) :=
-      SignExtendTruncLsb m (ZeroExtendTruncLsb 32 e).
-
-    Definition Trunc32Unsigned m n (e: Bit n @# ty) :=
-      ZeroExtendTruncLsb m (ZeroExtendTruncLsb 32 e).
-
-    Definition Sub n (e1 e2: Bit n @# ty) :=
-      e1 + ~e2 + $1.
+    Definition baseOutputXform (inp: BaseOutput @# ty): FuncOutput ## ty :=
+      ( LETC memOp : MemOpInfo <-
+                       STRUCT {
+                           "op" ::= ITE (inp @% "store?") $StOp $LdOp;
+                           "size" ::= inp @% "memSize";
+                           "MC" ::= inp @% "ldPerms" @% "MC";
+                           "LM" ::= inp @% "ldPerms" @% "LM";
+                           "LG" ::= inp @% "ldPerms" @% "LG";
+                           "sign?" ::= inp @% "ldSigned?";
+                           "cap?" ::= inp @% "memCap?" };
+        LETC cd : FullCapWithTag <-
+                    STRUCT {
+                        "tag" ::= inp @% "cdTag";
+                        "cap" ::= inp @% "cdCap";
+                        "val" ::= (IF (inp @% "exception?") || (inp @% "interrupt?")
+                                   then inp @% "exceptionCause"
+                                   else inp @% "cdVal") };
+        RetE (STRUCT {
+                  "data" ::= #cd;
+                  "pcCapOrMemOp" ::= ITE (inp @% "mem?")
+                                       (ZeroExtendTruncLsb CapSz (pack #memOp))
+                                       (inp @% "pcCap");
+                  "addr" ::= (inp @% "pcMemAddr");
+                  "wb?" ::= inp @% "wb?";
+                  "mayChangePc?" ::= inp @% "mayChangePc?";
+                  "taken?" ::= inp @% "taken?";
+                  "changePcCap?" ::= inp @% "changePcCap?";
+                  "mem?" ::= inp @% "mem?";
+                  "exception?" ::= inp @% "exception?";
+                  "exceptionCausePc?" ::= inp @% "exceptionCausePc?";
+                  "interrupt?" ::= inp @% "interrupt?";
+                  "changeIe?" ::= inp @% "changeIe?";
+                  "newIe" ::= inp @% "newIe" } : FuncOutput @# ty) ).
   End ty.
 
-  Definition baseSpecEntries: list (InstEntry SpecOutput SpecOutput) := [
-      {|instName := "AddI";
-        xlens := [32; 64];
-        extensions := [Base];
-        uniqId := [fieldVal opcodeField (5'b"00100");
-                   fieldVal funct3Field (3'b"000")];
-        inputXform ty pc inst cs1 cs2 ie :=
-          ( RetE ((DefSpecOutput ty)
-                    @%[ "wb?" <- $$true ]
-                    @%[ "cdVal" <- (cs1 @% "val") + SignExtendTruncLsb Xlen (imm inst)]));
-        outputXform ty (res: SpecOutput @# ty) :=
-          ( RetE (mkIntReg (res @% "cdVal") (res @% "takenPcCap") (res @% "takenPc")));
-        instProperties := {| hasCs1 := true; hasCs2 := false; implicit := 0 |}
-      |};
-      {|instName := "SLTI";
-        xlens := [32; 64];
-        extensions := [Base];
-        uniqId := [fieldVal opcodeField (5'b"00100");
-                   fieldVal funct3Field (3'b"010")];
-        inputXform ty pc inst cs1 cs2 ie :=
-          ( LETC in1 <- SignExtend 1 (cs1 @% "val");
-            LETC in2 <- SignExtendTruncLsb (Xlen + 1) (imm inst);
-            LETC res <- #in1 - #in2;
-            LETC msb <- UniBit (TruncMsb Xlen 1) #res;
-            RetE ((DefSpecOutput ty)
-                    @%[ "wb?" <- $$true ]
-                    @%[ "cdVal" <- ZeroExtendTruncLsb Xlen #msb]));
-        outputXform ty (res: SpecOutput @# ty) :=
-          ( RetE (mkIntReg (res @% "cdVal") (res @% "takenPcCap") (res @% "takenPc")));
-        instProperties := {| hasCs1 := true; hasCs2 := false; implicit := 0 |}
-      |};
-      {|instName := "SLTIU";
-        xlens := [32; 64];
-        extensions := [Base];
-        uniqId := [fieldVal opcodeField (5'b"00100");
-                   fieldVal funct3Field (3'b"011")];
-        inputXform ty pc inst cs1 cs2 ie :=
-          ( LETC in1 <- ZeroExtend 1 (cs1 @% "val");
-            LETC in2 <- ZeroExtendTruncLsb (Xlen + 1) (imm inst);
-            LETC res <- #in1 - #in2;
-            LETC msb <- UniBit (TruncMsb Xlen 1) #res;
-            RetE ((DefSpecOutput ty)
-                    @%[ "wb?" <- $$true ]
-                    @%[ "cdVal" <- ZeroExtendTruncLsb Xlen #msb]));
-        outputXform ty (res: SpecOutput @# ty) :=
-          ( RetE (mkIntReg (res @% "cdVal") (res @% "takenPcCap") (res @% "takenPc")));
-        instProperties := {| hasCs1 := true; hasCs2 := false; implicit := 0 |}
-      |};
-      {|instName := "XorI";
-        xlens := [32; 64];
-        extensions := [Base];
-        uniqId := [fieldVal opcodeField (5'b"00100");
-                   fieldVal funct3Field (3'b"100")];
-        inputXform ty pc inst cs1 cs2 ie :=
-          ( RetE ((DefSpecOutput ty)
-                    @%[ "wb?" <- $$true ]
-                    @%[ "cdVal" <- ((cs1 @% "val") .^ (SignExtendTruncLsb Xlen (imm inst))) ]));
-        outputXform ty (res: SpecOutput @# ty) :=
-          ( RetE (mkIntReg (res @% "cdVal") (res @% "takenPcCap") (res @% "takenPc")));
-        instProperties := {| hasCs1 := true; hasCs2 := false; implicit := 0 |}
-      |};
-      {|instName := "OrI";
-        xlens := [32; 64];
-        extensions := [Base];
-        uniqId := [fieldVal opcodeField (5'b"00100");
-                   fieldVal funct3Field (3'b"110")];
-        inputXform ty pc inst cs1 cs2 ie :=
-          ( RetE ((DefSpecOutput ty)
-                    @%[ "wb?" <- $$true ]
-                    @%[ "cdVal" <- ((cs1 @% "val") .| (SignExtendTruncLsb Xlen (imm inst))) ]));
-        outputXform ty (res: SpecOutput @# ty) :=
-          ( RetE (mkIntReg (res @% "cdVal") (res @% "takenPcCap") (res @% "takenPc")));
-        instProperties := {| hasCs1 := true; hasCs2 := false; implicit := 0 |}
-      |};
-      {|instName := "AndI";
-        xlens := [32; 64];
-        extensions := [Base];
-        uniqId := [fieldVal opcodeField (5'b"00100");
-                   fieldVal funct3Field (3'b"111")];
-        inputXform ty pc inst cs1 cs2 ie :=
-          ( RetE ((DefSpecOutput ty)
-                    @%[ "wb?" <- $$true ]
-                    @%[ "cdVal" <- ((cs1 @% "val") .& (SignExtendTruncLsb Xlen (imm inst))) ]));
-        outputXform ty (res: SpecOutput @# ty) :=
-          ( RetE (mkIntReg (res @% "cdVal") (res @% "takenPcCap") (res @% "takenPc")));
-        instProperties := {| hasCs1 := true; hasCs2 := false; implicit := 0 |}
-      |};
-      {|instName := "SLLI";
-        xlens := [32];
-        extensions := [Base];
-        uniqId := [fieldVal opcodeField (5'b"00100");
-                   fieldVal funct3Field (3'b"001");
-                   fieldVal funct7Field (7'b"0000000")];
-        inputXform ty pc inst cs1 cs2 ie :=
-          ( RetE ((DefSpecOutput ty)
-                    @%[ "wb?" <- $$true ]
-                    @%[ "cdVal" <- ((cs1 @% "val") <<
-                                      (ZeroExtendTruncLsb (Nat.log2_up Xlen) (imm inst)))]));
-        outputXform ty (res: SpecOutput @# ty) :=
-          ( RetE (mkIntReg (res @% "cdVal") (res @% "takenPcCap") (res @% "takenPc")));
-        instProperties := {| hasCs1 := true; hasCs2 := false; implicit := 0 |}
-      |};
-      {|instName := "SRLI";
-        xlens := [32];
-        extensions := [Base];
-        uniqId := [fieldVal opcodeField (5'b"00100");
-                   fieldVal funct3Field (3'b"101");
-                   fieldVal funct7Field (7'b"0000000")];
-        inputXform ty pc inst cs1 cs2 ie :=
-          ( RetE ((DefSpecOutput ty)
-                    @%[ "wb?" <- $$true ]
-                    @%[ "cdVal" <- UniBit (TruncLsb Xlen 1)
-                                     ((ZeroExtend 1 (cs1 @% "val")) >>>
+  Definition aluInsts: InstEntryFull BaseOutput :=
+    {|xlens := [32; 64];
+      extension := Base;
+      instEntries := [
+        {|instName := "AddI";
+          uniqId := [fieldVal opcodeField (5'b"00100");
+                     fieldVal funct3Field (3'b"000")];
+          inputXform ty pc inst cs1 cs2 ie :=
+            ( RetE ((DefBaseOutput ty)
+                      @%[ "wb?" <- $$true ]
+                      @%[ "cdVal" <- (cs1 @% "val") + SignExtendTruncLsb Xlen (imm inst)]));
+          instProperties := {| hasCs1 := true; hasCs2 := false; implicit := 0 |}
+        |};
+        {|instName := "SLTI";
+          uniqId := [fieldVal opcodeField (5'b"00100");
+                     fieldVal funct3Field (3'b"010")];
+          inputXform ty pc inst cs1 cs2 ie :=
+            ( LETC in1 <- SignExtend 1 (cs1 @% "val");
+              LETC in2 <- SignExtendTruncLsb (Xlen + 1) (imm inst);
+              LETC res <- #in1 - #in2;
+              LETC msb <- UniBit (TruncMsb Xlen 1) #res;
+              RetE ((DefBaseOutput ty)
+                      @%[ "wb?" <- $$true ]
+                      @%[ "cdVal" <- ZeroExtendTruncLsb Xlen #msb]));
+          instProperties := {| hasCs1 := true; hasCs2 := false; implicit := 0 |}
+        |};
+        {|instName := "SLTIU";
+          uniqId := [fieldVal opcodeField (5'b"00100");
+                     fieldVal funct3Field (3'b"011")];
+          inputXform ty pc inst cs1 cs2 ie :=
+            ( LETC in1 <- ZeroExtend 1 (cs1 @% "val");
+              LETC in2 <- ZeroExtendTruncLsb (Xlen + 1) (imm inst);
+              LETC res <- #in1 - #in2;
+              LETC msb <- UniBit (TruncMsb Xlen 1) #res;
+              RetE ((DefBaseOutput ty)
+                      @%[ "wb?" <- $$true ]
+                      @%[ "cdVal" <- ZeroExtendTruncLsb Xlen #msb]));
+          instProperties := {| hasCs1 := true; hasCs2 := false; implicit := 0 |}
+        |};
+        {|instName := "XorI";
+          uniqId := [fieldVal opcodeField (5'b"00100");
+                     fieldVal funct3Field (3'b"100")];
+          inputXform ty pc inst cs1 cs2 ie :=
+            ( RetE ((DefBaseOutput ty)
+                      @%[ "wb?" <- $$true ]
+                      @%[ "cdVal" <- ((cs1 @% "val") .^ (SignExtendTruncLsb Xlen (imm inst))) ]));
+          instProperties := {| hasCs1 := true; hasCs2 := false; implicit := 0 |}
+        |};
+        {|instName := "OrI";
+          uniqId := [fieldVal opcodeField (5'b"00100");
+                     fieldVal funct3Field (3'b"110")];
+          inputXform ty pc inst cs1 cs2 ie :=
+            ( RetE ((DefBaseOutput ty)
+                      @%[ "wb?" <- $$true ]
+                      @%[ "cdVal" <- ((cs1 @% "val") .| (SignExtendTruncLsb Xlen (imm inst))) ]));
+          instProperties := {| hasCs1 := true; hasCs2 := false; implicit := 0 |}
+        |};
+        {|instName := "AndI";
+          uniqId := [fieldVal opcodeField (5'b"00100");
+                     fieldVal funct3Field (3'b"111")];
+          inputXform ty pc inst cs1 cs2 ie :=
+            ( RetE ((DefBaseOutput ty)
+                      @%[ "wb?" <- $$true ]
+                      @%[ "cdVal" <- ((cs1 @% "val") .& (SignExtendTruncLsb Xlen (imm inst))) ]));
+          instProperties := {| hasCs1 := true; hasCs2 := false; implicit := 0 |}
+        |};
+        {|instName := "SLLI";
+          uniqId := [fieldVal opcodeField (5'b"00100");
+                     fieldVal funct3Field (3'b"001");
+                     if Xlen =? 32
+                     then fieldVal funct7Field (7'b"0000000")
+                     else fieldVal funct6Field (6'b"000000")];
+          inputXform ty pc inst cs1 cs2 ie :=
+            ( RetE ((DefBaseOutput ty)
+                      @%[ "wb?" <- $$true ]
+                      @%[ "cdVal" <- ((cs1 @% "val") <<
                                         (ZeroExtendTruncLsb (Nat.log2_up Xlen) (imm inst)))]));
-        outputXform ty (res: SpecOutput @# ty) :=
-          ( RetE (mkIntReg (res @% "cdVal") (res @% "takenPcCap") (res @% "takenPc")));
-        instProperties := {| hasCs1 := true; hasCs2 := false; implicit := 0 |}
-      |};
-      {|instName := "SRAI";
-        xlens := [32];
-        extensions := [Base];
-        uniqId := [fieldVal opcodeField (5'b"00100");
-                   fieldVal funct3Field (3'b"101");
-                   fieldVal funct7Field (7'b"0100000")];
+          instProperties := {| hasCs1 := true; hasCs2 := false; implicit := 0 |}
+        |};
+        {|instName := "SRLI";
+          uniqId := [fieldVal opcodeField (5'b"00100");
+                     fieldVal funct3Field (3'b"101");
+                     if Xlen =? 32
+                     then fieldVal funct7Field (7'b"0000000")
+                     else fieldVal funct6Field (6'b"000000")];
+          inputXform ty pc inst cs1 cs2 ie :=
+            ( RetE ((DefBaseOutput ty)
+                      @%[ "wb?" <- $$true ]
+                      @%[ "cdVal" <- UniBit (TruncLsb Xlen 1)
+                                       ((ZeroExtend 1 (cs1 @% "val")) >>>
+                                          (ZeroExtendTruncLsb (Nat.log2_up Xlen) (imm inst)))]));
+          instProperties := {| hasCs1 := true; hasCs2 := false; implicit := 0 |}
+        |};
+        {|instName := "SRAI";
+          uniqId := [fieldVal opcodeField (5'b"00100");
+                     fieldVal funct3Field (3'b"101");
+                     if Xlen =? 32
+                     then fieldVal funct7Field (7'b"0100000")
+                     else fieldVal funct6Field (6'b"010000")];
+          inputXform ty pc inst cs1 cs2 ie :=
+            ( RetE ((DefBaseOutput ty)
+                      @%[ "wb?" <- $$true ]
+                      @%[ "cdVal" <- UniBit (TruncLsb Xlen 1)
+                                       ((SignExtend 1 (cs1 @% "val")) >>>
+                                          (ZeroExtendTruncLsb (Nat.log2_up Xlen) (imm inst)))]));
+          instProperties := {| hasCs1 := true; hasCs2 := false; implicit := 0 |}
+        |};
+        {|instName := "Add";
+          uniqId := [fieldVal opcodeField (5'b"01100");
+                     fieldVal funct3Field (3'b"000");
+                     fieldVal funct7Field (7'b"0000000")];
+          inputXform ty pc inst cs1 cs2 ie :=
+            ( RetE ((DefBaseOutput ty)
+                      @%[ "wb?" <- $$true ]
+                      @%[ "cdVal" <- (cs1 @% "val") + (cs2 @% "val")]));
+          instProperties := {| hasCs1 := true; hasCs2 := true; implicit := 0 |}
+        |};
+        {|instName := "Sub";
+          uniqId := [fieldVal opcodeField (5'b"01100");
+                     fieldVal funct3Field (3'b"000");
+                     fieldVal funct7Field (7'b"0100000")];
+          inputXform ty pc inst cs1 cs2 ie :=
+            ( RetE ((DefBaseOutput ty)
+                      @%[ "wb?" <- $$true ]
+                      @%[ "cdVal" <- Sub (cs1 @% "val") (cs2 @% "val")]));
+          instProperties := {| hasCs1 := true; hasCs2 := true; implicit := 0 |}
+        |};
+        {|instName := "SLT";
+          uniqId := [fieldVal opcodeField (5'b"01100");
+                     fieldVal funct3Field (3'b"010");
+                     fieldVal funct7Field (7'b"0000000")];
+          inputXform ty pc inst cs1 cs2 ie :=
+            ( LETC in1 <- SignExtend 1 (cs1 @% "val");
+              LETC in2 <- SignExtend 1 (cs2 @% "val");
+              LETC res <- UniBit (TruncMsb Xlen 1) (#in1 + ~#in2 + $1);
+              RetE ((DefBaseOutput ty)
+                      @%[ "wb?" <- $$true ]
+                      @%[ "cdVal" <- ZeroExtendTruncLsb Xlen #res]));
+          instProperties := {| hasCs1 := true; hasCs2 := true; implicit := 0 |}
+        |};
+        {|instName := "SLTU";
+          uniqId := [fieldVal opcodeField (5'b"01100");
+                     fieldVal funct3Field (3'b"011");
+                     fieldVal funct7Field (7'b"0000000")];
+          inputXform ty pc inst cs1 cs2 ie :=
+            ( LETC in1 <- ZeroExtend 1 (cs1 @% "val");
+              LETC in2 <- ZeroExtend 1 (cs2 @% "val");
+              LETC res <- UniBit (TruncMsb Xlen 1) (#in1 + ~#in2 + $1);
+              RetE ((DefBaseOutput ty)
+                      @%[ "wb?" <- $$true ]
+                      @%[ "cdVal" <- ZeroExtendTruncLsb Xlen #res]));
+          instProperties := {| hasCs1 := true; hasCs2 := true; implicit := 0 |}
+        |};
+        {|instName := "Xor";
+          uniqId := [fieldVal opcodeField (5'b"01100");
+                     fieldVal funct3Field (3'b"100");
+                     fieldVal funct7Field (7'b"0000000")];
+          inputXform ty pc inst cs1 cs2 ie :=
+            ( RetE ((DefBaseOutput ty)
+                      @%[ "wb?" <- $$true ]
+                      @%[ "cdVal" <- (cs1 @% "val") .^ (cs2 @% "val")]));
+          instProperties := {| hasCs1 := true; hasCs2 := true; implicit := 0 |}
+        |};
+        {|instName := "Or";
+          uniqId := [fieldVal opcodeField (5'b"01100");
+                     fieldVal funct3Field (3'b"110");
+                     fieldVal funct7Field (7'b"0000000")];
+          inputXform ty pc inst cs1 cs2 ie :=
+            ( RetE ((DefBaseOutput ty)
+                      @%[ "wb?" <- $$true ]
+                      @%[ "cdVal" <- (cs1 @% "val") .| (cs2 @% "val")]));
+          instProperties := {| hasCs1 := true; hasCs2 := true; implicit := 0 |}
+        |};
+        {|instName := "And";
+          uniqId := [fieldVal opcodeField (5'b"01100");
+                     fieldVal funct3Field (3'b"111");
+                     fieldVal funct7Field (7'b"0000000")];
+          inputXform ty pc inst cs1 cs2 ie :=
+            ( RetE ((DefBaseOutput ty)
+                      @%[ "wb?" <- $$true ]
+                      @%[ "cdVal" <- (cs1 @% "val") .& (cs2 @% "val")]));
+          instProperties := {| hasCs1 := true; hasCs2 := true; implicit := 0 |}
+        |};
+        {|instName := "SLL";
+          uniqId := [fieldVal opcodeField (5'b"01100");
+                     fieldVal funct3Field (3'b"001");
+                     fieldVal funct7Field (7'b"0000000")];
+          inputXform ty pc inst cs1 cs2 ie :=
+            ( RetE ((DefBaseOutput ty)
+                      @%[ "wb?" <- $$true ]
+                      @%[ "cdVal" <- (cs1 @% "val") <<
+                                       (ZeroExtendTruncLsb (Nat.log2_up Xlen) (cs2 @% "val"))]));
+          instProperties := {| hasCs1 := true; hasCs2 := true; implicit := 0 |}
+        |};
+        {|instName := "SRL";
+          uniqId := [fieldVal opcodeField (5'b"01100");
+                     fieldVal funct3Field (3'b"101");
+                     fieldVal funct7Field (7'b"0000000")];
+          inputXform ty pc inst cs1 cs2 ie :=
+            ( RetE ((DefBaseOutput ty)
+                      @%[ "wb?" <- $$true ]
+                      @%[ "cdVal" <- UniBit (TruncLsb Xlen 1)
+                                       ((ZeroExtend 1 (cs1 @% "val")) >>>
+                                          (ZeroExtendTruncLsb (Nat.log2_up Xlen) (cs2 @% "val")))]));
+          instProperties := {| hasCs1 := true; hasCs2 := true; implicit := 0 |}
+        |};
+        {|instName := "SRA";
+          uniqId := [fieldVal opcodeField (5'b"01100");
+                     fieldVal funct3Field (3'b"101");
+                     fieldVal funct7Field (7'b"0100000")];
+          inputXform ty pc inst cs1 cs2 ie :=
+            ( RetE ((DefBaseOutput ty)
+                      @%[ "wb?" <- $$true ]
+                      @%[ "cdVal" <- UniBit (TruncLsb Xlen 1)
+                                       ((SignExtend 1 (cs1 @% "val")) >>>
+                                          (ZeroExtendTruncLsb (Nat.log2_up Xlen) (cs2 @% "val")))]));
+          instProperties := {| hasCs1 := true; hasCs2 := true; implicit := 0 |}
+        |}
+      ]
+    |}.
+
+  Definition alu64Insts: InstEntryFull BaseOutput :=
+    {|xlens := [64];
+      extension := Base;
+      instEntries := [
+        {|instName := "AddIW";
+          uniqId := [fieldVal opcodeField (5'b"00110");
+                     fieldVal funct3Field (3'b"000")];
+          inputXform ty pc inst cs1 cs2 ie :=
+            ( RetE ((DefBaseOutput ty)
+                      @%[ "wb?" <- $$true ]
+                      @%[ "cdVal" <- Trunc32Signed Xlen ((cs1 @% "val") + SignExtendTruncLsb Xlen (imm inst))]));
+          instProperties := {| hasCs1 := true; hasCs2 := false; implicit := 0 |}
+        |};
+        {|instName := "SLLIW";
+          uniqId := [fieldVal opcodeField (5'b"00110");
+                     fieldVal funct3Field (3'b"001");
+                     fieldVal funct7Field (7'b"0000000")];
+          inputXform ty pc inst cs1 cs2 ie :=
+            ( RetE ((DefBaseOutput ty)
+                      @%[ "wb?" <- $$true ]
+                      @%[ "cdVal" <- Trunc32Signed Xlen ((cs1 @% "val") <<
+                                                           (ZeroExtendTruncLsb (Nat.log2_up Xlen) (imm inst)))]));
+          instProperties := {| hasCs1 := true; hasCs2 := false; implicit := 0 |}
+        |};
+        {|instName := "SRLIW";
+          uniqId := [fieldVal opcodeField (5'b"00110");
+                     fieldVal funct3Field (3'b"101");
+                     fieldVal funct7Field (7'b"0000000")];
+          inputXform ty pc inst cs1 cs2 ie :=
+            ( RetE ((DefBaseOutput ty)
+                      @%[ "wb?" <- $$true ]
+                      @%[ "cdVal" <- (Trunc32Unsigned Xlen (cs1 @% "val")) >>>
+                                       (ZeroExtendTruncLsb (Nat.log2_up Xlen) (imm inst))]));
+          instProperties := {| hasCs1 := true; hasCs2 := false; implicit := 0 |}
+        |};
+        {|instName := "SRAIW";
+          uniqId := [fieldVal opcodeField (5'b"00110");
+                     fieldVal funct3Field (3'b"101");
+                     fieldVal funct7Field (7'b"0100000")];
+          inputXform ty pc inst cs1 cs2 ie :=
+            ( RetE ((DefBaseOutput ty)
+                      @%[ "wb?" <- $$true ]
+                      @%[ "cdVal" <- (Trunc32Signed Xlen (cs1 @% "val")) >>>
+                                       (ZeroExtendTruncLsb (Nat.log2_up Xlen) (imm inst))]));
+          instProperties := {| hasCs1 := true; hasCs2 := false; implicit := 0 |}
+        |};
+        {|instName := "AddW";
+          uniqId := [fieldVal opcodeField (5'b"01110");
+                     fieldVal funct3Field (3'b"000");
+                     fieldVal funct7Field (7'b"0000000")];
+          inputXform ty pc inst cs1 cs2 ie :=
+            ( RetE ((DefBaseOutput ty)
+                      @%[ "wb?" <- $$true ]
+                      @%[ "cdVal" <- Trunc32Signed Xlen ((cs1 @% "val") + (cs2 @% "val"))]));
+          instProperties := {| hasCs1 := true; hasCs2 := true; implicit := 0 |}
+        |};
+        {|instName := "SubW";
+          uniqId := [fieldVal opcodeField (5'b"01110");
+                     fieldVal funct3Field (3'b"000");
+                     fieldVal funct7Field (7'b"0100000")];
+          inputXform ty pc inst cs1 cs2 ie :=
+            ( RetE ((DefBaseOutput ty)
+                      @%[ "wb?" <- $$true ]
+                      @%[ "cdVal" <- Trunc32Signed Xlen (Sub (cs1 @% "val") (cs2 @% "val"))]));
+          instProperties := {| hasCs1 := true; hasCs2 := true; implicit := 0 |}
+        |};
+        {|instName := "SLLW";
+          uniqId := [fieldVal opcodeField (5'b"01110");
+                     fieldVal funct3Field (3'b"001");
+                     fieldVal funct7Field (7'b"0000000")];
+          inputXform ty pc inst cs1 cs2 ie :=
+            ( RetE ((DefBaseOutput ty)
+                      @%[ "wb?" <- $$true ]
+                      @%[ "cdVal" <- Trunc32Signed Xlen
+                                       ((cs1 @% "val") <<
+                                          (ZeroExtendTruncLsb (Nat.log2_up Xlen) (cs2 @% "val")))]));
+          instProperties := {| hasCs1 := true; hasCs2 := true; implicit := 0 |}
+        |};
+        {|instName := "SRLW";
+          uniqId := [fieldVal opcodeField (5'b"01110");
+                     fieldVal funct3Field (3'b"101");
+                     fieldVal funct7Field (7'b"0000000")];
+          inputXform ty pc inst cs1 cs2 ie :=
+            ( RetE ((DefBaseOutput ty)
+                      @%[ "wb?" <- $$true ]
+                      @%[ "cdVal" <- (Trunc32Unsigned Xlen (cs1 @% "val")) >>>
+                                       (ZeroExtendTruncLsb (Nat.log2_up Xlen) (cs2 @% "val"))]));
+          instProperties := {| hasCs1 := true; hasCs2 := true; implicit := 0 |}
+        |};
+        {|instName := "SRAW";
+          uniqId := [fieldVal opcodeField (5'b"01110");
+                     fieldVal funct3Field (3'b"101");
+                     fieldVal funct7Field (7'b"0100000")];
+          inputXform ty pc inst cs1 cs2 ie :=
+            ( RetE ((DefBaseOutput ty)
+                      @%[ "wb?" <- $$true ]
+                      @%[ "cdVal" <- (Trunc32Signed Xlen (cs1 @% "val")) >>>
+                                       (ZeroExtendTruncLsb (Nat.log2_up Xlen) (cs2 @% "val"))]));
+          instProperties := {| hasCs1 := true; hasCs2 := true; implicit := 0 |}
+        |}
+      ]
+    |}.
+
+  Definition capInsts: InstEntryFull BaseOutput :=
+    {|xlens := [32; 64];
+      extension := Base;
+      instEntries := [
+        {|instName := "AUICGP";
+          uniqId := [fieldVal opcodeField (truncMsb (7'h"7b"))];
+          inputXform ty pc inst cs1 cs2 ie :=
+            ( LETC newAddr <- (cs1 @% "val") + SignExtendTruncLsb Xlen ({< auiLuiOffset inst, $$(wzero 11) >});
+              LETE baseTop <- getCapBaseTop capAccessors (cs1 @% "cap") (cs1 @% "val");
+              LETC baseBound <- #newAddr >= (#baseTop @% "base");
+              LETC topBound <- (ZeroExtend 1 #newAddr) + $1 <= (#baseTop @% "top");
+              RetE ((DefBaseOutput ty)
+                      @%[ "wb?" <- $$true ]
+                      @%[ "cdTag" <- (cs1 @% "tag") && !isSealed capAccessors (cs1 @% "cap") && (#baseBound && #topBound) ]
+                      @%[ "cdCap" <- cs1 @% "cap" ]
+                      @%[ "cdVal" <- #newAddr ]));
+          instProperties := {| hasCs1 := false; hasCs2 := false; implicit := 3 |}
+        |};
+        {|instName := "AUIPCC";
+          uniqId := [fieldVal opcodeField (truncMsb (7'h"17"))];
+          inputXform ty pc inst cs1 cs2 ie :=
+            ( LETC newAddr <- (pc @% "val") + SignExtendTruncLsb Xlen ({< auiLuiOffset inst, $$(wzero 11) >});
+              LETE baseTop <- getCapBaseTop capAccessors (pc @% "cap") (pc @% "val");
+              LETC baseBound <- #newAddr >= (#baseTop @% "base");
+              LETC topBound <- ZeroExtend 1 #newAddr + $1 <= #baseTop @% "top";
+              RetE ((DefBaseOutput ty)
+                      @%[ "wb?" <- $$true ]
+                      @%[ "cdTag" <- #baseBound && #topBound ]
+                      @%[ "cdCap" <- pc @% "cap" ]
+                      @%[ "cdVal" <- #newAddr ]));
+          instProperties := {| hasCs1 := false; hasCs2 := false; implicit := 3 |}
+        |};
+        {|instName := "CAndPerm";
+          uniqId := [fieldVal opcodeField (truncMsb (7'h"5b"));
+                     fieldVal funct3Field (3'h"0");
+                     fieldVal funct7Field (7'h"d")];
+          inputXform ty pc inst cs1 cs2 ie :=
+            ( LETE perms <- getCapPerms capAccessors (cs1 @% "cap");
+              LETC newPerms <- unpack CapPerms (ZeroExtendTruncLsb (size CapPerms)
+                                                  ((ZeroExtendTruncLsb Xlen (pack #perms)) .& (cs2 @% "val")));
+              LETE newCap <- setCapPerms capAccessors (cs1 @% "cap") #newPerms;
+              RetE ((DefBaseOutput ty)
+                      @%[ "wb?" <- $$true ]
+                      @%[ "cdTag" <- cs1 @% "tag" ]
+                      @%[ "cdCap" <- #newCap ]
+                      @%[ "cdVal" <- cs1 @% "val" ]));
+          instProperties := {| hasCs1 := true; hasCs2 := true; implicit := 0 |}
+        |};
+        {|instName := "CClearTag";
+          uniqId := [fieldVal opcodeField (truncMsb (7'h"5b"));
+                     fieldVal funct3Field (3'h"0");
+                     fieldVal rs2FixedField (5'h"b");
+                     fieldVal funct7Field (7'h"7f")];
+          inputXform ty pc inst cs1 cs2 ie :=
+            ( RetE ((DefBaseOutput ty)
+                      @%[ "wb?" <- $$true ]
+                      @%[ "cdTag" <- $$false ]
+                      @%[ "cdCap" <- cs1 @% "cap" ]
+                      @%[ "cdVal" <- cs1 @% "val" ]));
+          instProperties := {| hasCs1 := true; hasCs2 := false; implicit := 0 |}
+        |};
+        {|instName := "CGetAddr";
+          uniqId := [fieldVal opcodeField (truncMsb (7'h"5b"));
+                     fieldVal funct3Field (3'h"0");
+                     fieldVal rs2FixedField (5'h"f");
+                     fieldVal funct7Field (7'h"7f")];
+          inputXform ty pc inst cs1 cs2 ie :=
+            ( RetE ((DefBaseOutput ty)
+                      @%[ "wb?" <- $$true ]
+                      @%[ "cdVal" <- cs1 @% "val" ]));
+          instProperties := {| hasCs1 := true; hasCs2 := false; implicit := 0 |}
+        |};
+        {|instName := "CGetBase";
+          uniqId := [fieldVal opcodeField (truncMsb (7'h"5b"));
+                     fieldVal funct3Field (3'h"0");
+                     fieldVal rs2FixedField (5'h"2");
+                     fieldVal funct7Field (7'h"7f")];
+          inputXform ty pc inst cs1 cs2 ie :=
+            ( LETE baseTop <- getCapBaseTop capAccessors (cs1 @% "cap") (cs1 @% "val");
+              RetE ((DefBaseOutput ty)
+                      @%[ "wb?" <- $$true ]
+                      @%[ "cdVal" <- #baseTop @% "base" ]));
+          instProperties := {| hasCs1 := true; hasCs2 := false; implicit := 0 |}
+        |};
+        {|instName := "CGetHigh";
+          uniqId := [fieldVal opcodeField (truncMsb (7'h"5b"));
+                     fieldVal funct3Field (3'h"0");
+                     fieldVal rs2FixedField (5'h"17");
+                     fieldVal funct7Field (7'h"7f")];
+          inputXform ty pc inst cs1 cs2 ie :=
+            ( RetE ((DefBaseOutput ty)
+                      @%[ "wb?" <- $$true ]
+                      @%[ "cdVal" <- cs1 @% "cap" ]));
+          instProperties := {| hasCs1 := true; hasCs2 := false; implicit := 0 |}
+        |};
+        {|instName := "CGetLen";
+          uniqId := [fieldVal opcodeField (truncMsb (7'h"5b"));
+                     fieldVal funct3Field (3'h"0");
+                     fieldVal rs2FixedField (5'h"3");
+                     fieldVal funct7Field (7'h"7f")];
+          inputXform ty pc inst cs1 cs2 ie :=
+            ( LETE baseTop <- getCapBaseTop capAccessors (cs1 @% "cap") (cs1 @% "val");
+              LETC len <- (#baseTop @% "top") - ZeroExtend 1 (#baseTop @% "base");
+              LETC lenMsb <- unpack Bool (UniBit (TruncMsb Xlen 1) #len);
+              LETC lenLsb <- UniBit (TruncLsb Xlen 1) #len;
+              RetE ((DefBaseOutput ty)
+                      @%[ "wb?" <- $$true ]
+                      @%[ "cdVal" <- ITE #lenMsb $$(wones Xlen) #lenLsb ]));
+          instProperties := {| hasCs1 := true; hasCs2 := false; implicit := 0 |}
+        |};
+        {|instName := "CGetPerm";
+          uniqId := [fieldVal opcodeField (truncMsb (7'h"5b"));
+                     fieldVal funct3Field (3'h"0");
+                     fieldVal rs2FixedField (5'h"0");
+                     fieldVal funct7Field (7'h"7f")];
+          inputXform ty pc inst cs1 cs2 ie :=
+            ( LETE perms <- getCapPerms capAccessors (cs1 @% "cap");
+              RetE ((DefBaseOutput ty)
+                      @%[ "wb?" <- $$true ]
+                      @%[ "cdVal" <- ZeroExtendTruncLsb Xlen (pack #perms) ]));
+          instProperties := {| hasCs1 := true; hasCs2 := false; implicit := 0 |}
+        |};
+        {|instName := "CGetTag";
+          uniqId := [fieldVal opcodeField (truncMsb (7'h"5b"));
+                     fieldVal funct3Field (3'h"0");
+                     fieldVal rs2FixedField (5'h"4");
+                     fieldVal funct7Field (7'h"7f")];
+          inputXform ty pc inst cs1 cs2 ie :=
+            ( RetE ((DefBaseOutput ty)
+                      @%[ "wb?" <- $$true ]
+                      @%[ "cdVal" <- ZeroExtendTruncLsb Xlen (pack (cs1 @% "tag")) ]));
+          instProperties := {| hasCs1 := true; hasCs2 := false; implicit := 0 |}
+        |};
+        {|instName := "CGetTop";
+          uniqId := [fieldVal opcodeField (truncMsb (7'h"5b"));
+                     fieldVal funct3Field (3'h"0");
+                     fieldVal rs2FixedField (5'h"18");
+                     fieldVal funct7Field (7'h"7f")];
+          inputXform ty pc inst cs1 cs2 ie :=
+            ( LETE baseTop <- getCapBaseTop capAccessors (cs1 @% "cap") (cs1 @% "val");
+              LETC topMsb <- unpack Bool (UniBit (TruncMsb Xlen 1) (#baseTop @% "top"));
+              LETC topLsb <- UniBit (TruncLsb Xlen 1) (#baseTop @% "top");
+              RetE ((DefBaseOutput ty)
+                      @%[ "wb?" <- $$true ]
+                      @%[ "cdVal" <- ITE #topMsb $$(wones Xlen) #topLsb ]));
+          instProperties := {| hasCs1 := true; hasCs2 := false; implicit := 0 |}
+        |};
+        {|instName := "CGetType";
+          uniqId := [fieldVal opcodeField (truncMsb (7'h"5b"));
+                     fieldVal funct3Field (3'h"0");
+                     fieldVal rs2FixedField (5'h"1");
+                     fieldVal funct7Field (7'h"7f")];
+          inputXform ty pc inst cs1 cs2 ie :=
+            ( LETC oType <- getCapOType capAccessors (cs1 @% "cap");
+              RetE ((DefBaseOutput ty)
+                      @%[ "wb?" <- $$true ]
+                      @%[ "cdVal" <- ZeroExtendTruncLsb Xlen #oType ]));
+          instProperties := {| hasCs1 := true; hasCs2 := false; implicit := 0 |}
+        |};
+        {|instName := "CIncAddr";
+          uniqId := [fieldVal opcodeField (truncMsb (7'h"5b"));
+                     fieldVal funct3Field (3'h"0");
+                     fieldVal funct7Field (7'h"11")];
+          inputXform ty pc inst cs1 cs2 ie :=
+            ( LETC newAddr <- (cs1 @% "val") + (cs2 @% "val");
+              LETE baseTop <- getCapBaseTop capAccessors (cs1 @% "cap") (cs1 @% "val");
+              LETC baseBound <- #newAddr >= #baseTop @% "base";
+              LETC topBound <- ZeroExtend 1 #newAddr + $1 <= #baseTop @% "top";
+              RetE ((DefBaseOutput ty)
+                      @%[ "wb?" <- $$true ]
+                      @%[ "cdTag" <- (cs1 @% "tag") && !isSealed capAccessors (cs1 @% "val") && (#baseBound && #topBound) ]
+                      @%[ "cdCap" <- cs1 @% "cap" ]
+                      @%[ "cdVal" <- #newAddr ]));
+          instProperties := {| hasCs1 := true; hasCs2 := true; implicit := 0 |}
+        |};
+        {|instName := "CIncAddrImm";
+          uniqId := [fieldVal opcodeField (truncMsb (7'h"5b"));
+                     fieldVal funct3Field (3'h"1")];
+          inputXform ty pc inst cs1 cs2 ie :=
+            ( LETC newAddr <- (cs1 @% "val") + SignExtendTruncLsb Xlen (imm inst);
+              LETE baseTop <- getCapBaseTop capAccessors (cs1 @% "cap") (cs1 @% "val");
+              LETC baseBound <- #newAddr >= #baseTop @% "base";
+              LETC topBound <- ZeroExtend 1 #newAddr + $1 <= #baseTop @% "top";
+              RetE ((DefBaseOutput ty)
+                      @%[ "wb?" <- $$true ]
+                      @%[ "cdTag" <- (cs1 @% "tag") && !isSealed capAccessors (cs1 @% "val") && (#baseBound && #topBound) ]
+                      @%[ "cdCap" <- cs1 @% "cap" ]
+                      @%[ "cdVal" <- #newAddr ]));
+          instProperties := {| hasCs1 := true; hasCs2 := false; implicit := 0 |}
+        |};
+        {|instName := "CMove";
+          uniqId := [fieldVal opcodeField (truncMsb (7'h"5b"));
+                     fieldVal funct3Field (3'h"0");
+                     fieldVal rs2FixedField (5'h"a");
+                     fieldVal funct7Field (7'h"7f")];
+          inputXform ty pc inst cs1 cs2 ie :=
+            ( RetE ((DefBaseOutput ty)
+                      @%[ "wb?" <- $$true ]
+                      @%[ "cdTag" <- cs1 @% "tag" ]
+                      @%[ "cdCap" <- cs1 @% "cap" ]
+                      @%[ "cdVal" <- cs1 @% "val" ]));
+          instProperties := {| hasCs1 := true; hasCs2 := false; implicit := 0 |}
+        |};
+        {|instName := "CRepresentableAlignmentMask";
+          uniqId := [fieldVal opcodeField (truncMsb (7'h"5b"));
+                     fieldVal funct3Field (3'h"0");
+                     fieldVal rs2FixedField (5'h"9");
+                     fieldVal funct7Field (7'h"7f")];
+          inputXform ty pc inst cs1 cs2 ie :=
+            ( LETE capBounds <- getCapBounds capAccessors ($0) (cs1 @% "val");
+              LETC mask <- $$(wones Xlen) << (#capBounds @% "exp");
+              RetE ((DefBaseOutput ty)
+                      @%[ "wb?" <- $$true ]
+                      @%[ "cdVal" <- #mask ]));
+          instProperties := {| hasCs1 := true; hasCs2 := false; implicit := 0 |}
+        |};
+        {|instName := "CRoundRepresentableLength";
+          uniqId := [fieldVal opcodeField (truncMsb (7'h"5b"));
+                     fieldVal funct3Field (3'h"0");
+                     fieldVal rs2FixedField (5'h"8");
+                     fieldVal funct7Field (7'h"7f")];
+          inputXform ty pc inst cs1 cs2 ie :=
+            ( LETE capBounds <- getCapBounds capAccessors ($0) (cs1 @% "val");
+              LETC mask <- $$(wones Xlen) << (#capBounds @% "exp");
+              LETC repLen <- (cs1 @% "val" + ~#mask) .& #mask;
+              RetE ((DefBaseOutput ty)
+                      @%[ "wb?" <- $$true ]
+                      @%[ "cdVal" <- #repLen ]));
+          instProperties := {| hasCs1 := true; hasCs2 := false; implicit := 0 |}
+        |};
+        {|instName := "CSetAddr";
+          uniqId := [fieldVal opcodeField (truncMsb (7'h"5b"));
+                     fieldVal funct3Field (3'h"0");
+                     fieldVal funct7Field (7'h"10")];
+          inputXform ty pc inst cs1 cs2 ie :=
+            ( LETC newAddr <- cs2 @% "val";
+              LETE baseTop <- getCapBaseTop capAccessors (cs1 @% "cap") (cs1 @% "val");
+              LETC baseBound <- #newAddr >= (#baseTop @% "base");
+              LETC topBound <- ZeroExtend 1 #newAddr + $1 <= (#baseTop @% "top");
+              RetE ((DefBaseOutput ty)
+                      @%[ "wb?" <- $$true ]
+                      @%[ "cdTag" <- (cs1 @% "tag") && !isSealed capAccessors (cs1 @% "val") && (#baseBound && #topBound) ]
+                      @%[ "cdCap" <- cs1 @% "cap" ]
+                      @%[ "cdVal" <- #newAddr ]));
+          instProperties := {| hasCs1 := true; hasCs2 := true; implicit := 0 |}
+        |};
+        {|instName := "CSetBounds";
+          uniqId := [fieldVal opcodeField (truncMsb (7'h"5b"));
+                     fieldVal funct3Field (3'h"0");
+                     fieldVal funct7Field (7'h"8")];
+          inputXform ty pc inst cs1 cs2 ie :=
+            ( LETE baseTop <- getCapBaseTop capAccessors (cs1 @% "cap") (cs1 @% "val");
+              LETC baseBound <- (cs1 @% "val") >= (#baseTop @% "base");
+              LETC topBound <- (ZeroExtend 1 (cs1 @% "val") + ZeroExtend 1 (cs2 @% "val")) <= (#baseTop @% "top");
+              LETE capBounds <- getCapBounds capAccessors (cs1 @% "cap") (cs1 @% "val");
+              LETC newCap <- setCapBounds capAccessors (cs1 @% "cap") (#capBounds @% "B") (#capBounds @% "T") (#capBounds @% "exp");
+              RetE ((DefBaseOutput ty)
+                      @%[ "wb?" <- $$true ]
+                      @%[ "cdTag" <- (cs1 @% "tag") && !isSealed capAccessors (cs1 @% "val") && (#baseBound && #topBound) ]
+                      @%[ "cdCap" <- #newCap ]
+                      @%[ "cdVal" <- cs1 @% "val" ]));
+          instProperties := {| hasCs1 := true; hasCs2 := true; implicit := 0 |}
+        |};
+        {|instName := "CSetBoundsExact";
+          uniqId := [fieldVal opcodeField (truncMsb (7'h"5b"));
+                     fieldVal funct3Field (3'h"0");
+                     fieldVal funct7Field (7'h"9")];
+          inputXform ty pc inst cs1 cs2 ie :=
+            ( LETE baseTop <- getCapBaseTop capAccessors (cs1 @% "cap") (cs1 @% "val");
+              LETC baseBound <- (cs1 @% "val") >= (#baseTop @% "base");
+              LETC topBound <- (ZeroExtend 1 (cs1 @% "val") + ZeroExtend 1 (cs2 @% "val")) <= (#baseTop @% "top");
+              LETE capBounds <- getCapBounds capAccessors (cs1 @% "cap") (cs1 @% "val");
+              LETC newCap <- setCapBounds capAccessors (cs1 @% "cap") (#capBounds @% "B") (#capBounds @% "T") (#capBounds @% "exp");
+              RetE ((DefBaseOutput ty)
+                      @%[ "wb?" <- $$true ]
+                      @%[ "cdTag" <- (cs1 @% "tag") && !isSealed capAccessors (cs1 @% "val") && (#baseBound && #topBound) && (#capBounds @% "exact?")]
+                      @%[ "cdCap" <- #newCap ]
+                      @%[ "cdVal" <- cs1 @% "val" ]));
+          instProperties := {| hasCs1 := true; hasCs2 := true; implicit := 0 |}
+        |};
+        {|instName := "CSetBoundsImm";
+          uniqId := [fieldVal opcodeField (truncMsb (7'h"5b"));
+                     fieldVal funct3Field (3'h"2")];
+          inputXform ty pc inst cs1 cs2 ie :=
+            ( LETE baseTop <- getCapBaseTop capAccessors (cs1 @% "cap") (cs1 @% "val");
+              LETC baseBound <- (cs1 @% "val") >= (#baseTop @% "base");
+              LETC topBound <- (ZeroExtend 1 (cs1 @% "val") + ZeroExtendTruncLsb (Xlen + 1) (imm inst)) <= (#baseTop @% "top");
+              LETE capBounds <- getCapBounds capAccessors (cs1 @% "cap") (cs1 @% "val");
+              LETC newCap <- setCapBounds capAccessors (cs1 @% "cap") (#capBounds @% "B") (#capBounds @% "T") (#capBounds @% "exp");
+              RetE ((DefBaseOutput ty)
+                      @%[ "wb?" <- $$true ]
+                      @%[ "cdTag" <- (cs1 @% "tag") && !isSealed capAccessors (cs1 @% "val") && (#baseBound && #topBound) ]
+                      @%[ "cdCap" <- #newCap ]
+                      @%[ "cdVal" <- cs1 @% "val" ]));
+          instProperties := {| hasCs1 := true; hasCs2 := true; implicit := 0 |}
+        |};
+        {|instName := "CSetEqualExact";
+          uniqId := [fieldVal opcodeField (truncMsb (7'h"5b"));
+                     fieldVal funct3Field (3'h"0");
+                     fieldVal funct7Field (7'h"21")];
+          inputXform ty pc inst cs1 cs2 ie :=
+            ( LETC tagEq <- (cs1 @% "tag") == (cs2 @% "tag");
+              LETC capEq <- (cs1 @% "cap") == (cs2 @% "cap");
+              LETC valEq <- (cs1 @% "val") == (cs2 @% "val");
+              RetE ((DefBaseOutput ty)
+                      @%[ "wb?" <- $$true ]
+                      @%[ "cdVal" <- ZeroExtendTruncLsb Xlen (pack (#tagEq && #capEq && #valEq)) ]));
+          instProperties := {| hasCs1 := true; hasCs2 := true; implicit := 0 |}
+        |};
+        {|instName := "CSetHigh";
+          uniqId := [fieldVal opcodeField (truncMsb (7'h"5b"));
+                     fieldVal funct3Field (3'h"0");
+                     fieldVal funct7Field (7'h"16")];
+          inputXform ty pc inst cs1 cs2 ie :=
+            ( RetE ((DefBaseOutput ty)
+                      @%[ "wb?" <- $$true ]
+                      @%[ "cdTag" <- $$false ]
+                      @%[ "cdCap" <- cs2 @% "val" ]
+                      @%[ "cdVal" <- cs1 @% "val" ]));
+          instProperties := {| hasCs1 := true; hasCs2 := true; implicit := 0 |}
+        |};
+        {|instName := "CSub";
+          uniqId := [fieldVal opcodeField (truncMsb (7'h"5b"));
+                     fieldVal funct3Field (3'h"0");
+                     fieldVal funct7Field (7'h"14")];
+          inputXform ty pc inst cs1 cs2 ie :=
+            ( RetE ((DefBaseOutput ty)
+                      @%[ "wb?" <- $$true ]
+                      @%[ "cdVal" <- Sub (cs1 @% "val") (cs2 @% "val") ]));
+          instProperties := {| hasCs1 := true; hasCs2 := true; implicit := 0 |}
+        |};
+        {|instName := "CTestSubset";
+          uniqId := [fieldVal opcodeField (truncMsb (7'h"5b"));
+                     fieldVal funct3Field (3'h"0");
+                     fieldVal funct7Field (7'h"20")];
+          inputXform ty pc inst cs1 cs2 ie :=
+            ( LETE baseTop <- getCapBaseTop capAccessors (cs1 @% "cap") (cs1 @% "val");
+              LETE baseTop2 <- getCapBaseTop capAccessors (cs2 @% "cap") (cs2 @% "val");
+              LETC baseBound <- (#baseTop2 @% "base") >= (#baseTop @% "base");
+              LETC topBound <- (#baseTop2 @% "top") <= (#baseTop @% "top");
+              LETC tagEq <- (cs1 @% "tag") == (cs2 @% "tag");
+              LETE perms <- getCapPerms capAccessors (cs1 @% "cap");
+              LETE perms2 <- getCapPerms capAccessors (cs2 @% "cap");
+              LETC permsAnd <- (pack #perms .& pack #perms2);
+              LETC permsSub <- #permsAnd == pack #perms2;
+              RetE ((DefBaseOutput ty)
+                      @%[ "wb?" <- $$true ]
+                      @%[ "cdVal" <- ZeroExtendTruncLsb Xlen (pack (#baseBound && #topBound && #tagEq && #permsSub)) ]));
+          instProperties := {| hasCs1 := true; hasCs2 := true; implicit := 0 |}
+        |};
+        {|instName := "CSeal";
+          uniqId := [fieldVal opcodeField (truncMsb (7'h"5b"));
+                     fieldVal funct3Field (3'h"0");
+                     fieldVal funct7Field (7'h"b")];
+          inputXform ty pc inst cs1 cs2 ie :=
+            ( LETE baseTop2 <- getCapBaseTop capAccessors (cs2 @% "cap") (cs2 @% "val");
+              LETC baseBound <- (cs2 @% "val") >= (#baseTop2 @% "base");
+              LETC topBound <- ZeroExtend 1 (cs2 @% "val") + $1 <= (#baseTop2 @% "top");
+              LETE perms <- getCapPerms capAccessors (cs1 @% "cap");
+              LETE perms2 <- getCapPerms capAccessors (cs2 @% "cap");
+              LETE validSealAddr <- isSealAddr capAccessors (cs2 @% "val") (#perms @% "EX");
+              LETC newCap <- seal capAccessors (cs1 @% "cap") (ZeroExtendTruncLsb (CapOTypeSz capAccessors) (cs2 @% "val"));
+              RetE ((DefBaseOutput ty)
+                      @%[ "wb?" <- $$true ]
+                      @%[ "cdTag" <- (cs2 @% "tag") && !isSealed capAccessors (cs2 @% "cap") && (#baseBound && #topBound) &&
+                                       (cs1 @% "tag") && !isSealed capAccessors (cs1 @% "cap") && (#perms2 @% "SE") && #validSealAddr]
+                      @%[ "cdCap" <- #newCap ]
+                      @%[ "cdVal" <- cs1 @% "val" ]));
+          instProperties := {| hasCs1 := true; hasCs2 := true; implicit := 0 |}
+        |};
+        {|instName := "CUnseal";
+          uniqId := [fieldVal opcodeField (truncMsb (7'h"5b"));
+                     fieldVal funct3Field (3'h"0");
+                     fieldVal funct7Field (7'h"c")];
+          inputXform ty pc inst cs1 cs2 ie :=
+            ( LETE baseTop2 <- getCapBaseTop capAccessors (cs2 @% "cap") (cs2 @% "val");
+              LETC baseBound <- (cs2 @% "val") >= (#baseTop2 @% "base");
+              LETC topBound <- ZeroExtend 1 (cs2 @% "val") + $1 <= (#baseTop2 @% "top");
+              LETC oType <- getCapOType capAccessors (cs1 @% "cap");
+              LETC oTypeEq <- ZeroExtendTruncLsb Xlen #oType == (cs2 @% "val");
+              LETE perms <- getCapPerms capAccessors (cs1 @% "cap");
+              LETE perms2 <- getCapPerms capAccessors (cs2 @% "cap");
+              LETC newPerms <- #perms @%[ "GL" <- #perms @% "GL" && #perms2 @% "GL" ];
+              LETE newCapWithPerms <- setCapPerms capAccessors (cs1 @% "cap") #newPerms;
+              LETC newCap <- unseal capAccessors #newCapWithPerms;
+              RetE ((DefBaseOutput ty)
+                      @%[ "wb?" <- $$true ]
+                      @%[ "cdTag" <- (cs2 @% "tag") && !isSealed capAccessors (cs2 @% "cap") && (#baseBound && #topBound) &&
+                                       (cs1 @% "tag") && isSealed capAccessors (cs1 @% "cap") && (#perms2 @% "US") && #oTypeEq]
+                      @%[ "cdCap" <- #newCap ]
+                      @%[ "cdVal" <- cs1 @% "val" ]));
+          instProperties := {| hasCs1 := true; hasCs2 := true; implicit := 0 |}
+        |}
+      ]
+    |}.
+
+  Definition mkBranchInst (name: string) funct3Val (takenFn: forall {ty}, Data @# ty -> Data @# ty -> Bool ## ty) :=
+      {|instName := name;
+        uniqId := [fieldVal opcodeField (5'b"11000");
+                   fieldVal funct3Field funct3Val];
         inputXform ty pc inst cs1 cs2 ie :=
-          ( RetE ((DefSpecOutput ty)
-                    @%[ "wb?" <- $$true ]
-                    @%[ "cdVal" <- UniBit (TruncLsb Xlen 1)
-                                     ((SignExtend 1 (cs1 @% "val")) >>>
-                                        (ZeroExtendTruncLsb (Nat.log2_up Xlen) (imm inst)))]));
-        outputXform ty (res: SpecOutput @# ty) :=
-          ( RetE (mkIntReg (res @% "cdVal") (res @% "takenPcCap") (res @% "takenPc")));
-        instProperties := {| hasCs1 := true; hasCs2 := false; implicit := 0 |}
-      |};
-      {|instName := "SLLI";
-        xlens := [64];
-        extensions := [Base];
-        uniqId := [fieldVal opcodeField (5'b"00100");
-                   fieldVal funct3Field (3'b"001");
-                   fieldVal funct6Field (6'b"000000")];
-        inputXform ty pc inst cs1 cs2 ie :=
-          ( RetE ((DefSpecOutput ty)
-                    @%[ "wb?" <- $$true ]
-                    @%[ "cdVal" <- ((cs1 @% "val") <<
-                                      (ZeroExtendTruncLsb (Nat.log2_up Xlen) (imm inst)))]));
-        outputXform ty (res: SpecOutput @# ty) :=
-          ( RetE (mkIntReg (res @% "cdVal") (res @% "takenPcCap") (res @% "takenPc")));
-        instProperties := {| hasCs1 := true; hasCs2 := false; implicit := 0 |}
-      |};
-      {|instName := "SRLI";
-        xlens := [64];
-        extensions := [Base];
-        uniqId := [fieldVal opcodeField (5'b"00100");
-                   fieldVal funct3Field (3'b"101");
-                   fieldVal funct6Field (6'b"000000")];
-        inputXform ty pc inst cs1 cs2 ie :=
-          ( RetE ((DefSpecOutput ty)
-                    @%[ "wb?" <- $$true ]
-                    @%[ "cdVal" <- UniBit (TruncLsb Xlen 1)
-                                     ((ZeroExtend 1 (cs1 @% "val")) >>>
-                                        (ZeroExtendTruncLsb (Nat.log2_up Xlen) (imm inst)))]));
-        outputXform ty (res: SpecOutput @# ty) :=
-          ( RetE (mkIntReg (res @% "cdVal") (res @% "takenPcCap") (res @% "takenPc")));
-        instProperties := {| hasCs1 := true; hasCs2 := false; implicit := 0 |}
-      |};
-      {|instName := "SRAI";
-        xlens := [64];
-        extensions := [Base];
-        uniqId := [fieldVal opcodeField (5'b"00100");
-                   fieldVal funct3Field (3'b"101");
-                   fieldVal funct6Field (6'b"010000")];
-        inputXform ty pc inst cs1 cs2 ie :=
-          ( RetE ((DefSpecOutput ty)
-                    @%[ "wb?" <- $$true ]
-                    @%[ "cdVal" <- UniBit (TruncLsb Xlen 1)
-                                     ((SignExtend 1 (cs1 @% "val")) >>>
-                                        (ZeroExtendTruncLsb (Nat.log2_up Xlen) (imm inst)))]));
-        outputXform ty (res: SpecOutput @# ty) :=
-          ( RetE (mkIntReg (res @% "cdVal") (res @% "takenPcCap") (res @% "takenPc")));
-        instProperties := {| hasCs1 := true; hasCs2 := false; implicit := 0 |}
-      |};
-      {|instName := "Add";
-        xlens := [32; 64];
-        extensions := [Base];
-        uniqId := [fieldVal opcodeField (5'b"01100");
-                   fieldVal funct3Field (3'b"000");
-                   fieldVal funct7Field (7'b"0000000")];
-        inputXform ty pc inst cs1 cs2 ie :=
-          ( RetE ((DefSpecOutput ty)
-                    @%[ "wb?" <- $$true ]
-                    @%[ "cdVal" <- (cs1 @% "val") + (cs2 @% "val")]));
-        outputXform ty (res: SpecOutput @# ty) :=
-          ( RetE (mkIntReg (res @% "cdVal") (res @% "takenPcCap") (res @% "takenPc")));
+          ( LETC newAddr <- (pc @% "val") + SignExtendTruncLsb Xlen (branchOffset inst);
+            LETE taken <- takenFn (cs1 @% "val") (cs2 @% "val");
+            RetE ((DefBaseOutput ty)
+                    @%[ "mayChangePc?" <- $$true ]
+                    @%[ "taken?" <- #taken ]
+                    @%[ "pcMemAddr" <- #newAddr ]
+                    @%[ "exception?" <- if compressed
+                                        then $$false
+                                        else isNotZero (ZeroExtendTruncLsb 2 #newAddr) ]
+                    @%[ "exceptionCause" <- if compressed
+                                            then Const ty (natToWord Xlen 0)
+                                            else $InstMisaligned ]
+                    @%[ "exceptionCausePc?" <- $$true ]));
         instProperties := {| hasCs1 := true; hasCs2 := true; implicit := 0 |}
-      |};
-      {|instName := "Sub";
-        xlens := [32; 64];
-        extensions := [Base];
-        uniqId := [fieldVal opcodeField (5'b"01100");
-                   fieldVal funct3Field (3'b"000");
-                   fieldVal funct7Field (7'b"0100000")];
-        inputXform ty pc inst cs1 cs2 ie :=
-          ( RetE ((DefSpecOutput ty)
-                    @%[ "wb?" <- $$true ]
-                    @%[ "cdVal" <- Sub (cs1 @% "val") (cs2 @% "val")]));
-        outputXform ty (res: SpecOutput @# ty) :=
-          ( RetE (mkIntReg (res @% "cdVal") (res @% "takenPcCap") (res @% "takenPc")));
-        instProperties := {| hasCs1 := true; hasCs2 := true; implicit := 0 |}
-      |};
-      {|instName := "SLT";
-        xlens := [32; 64];
-        extensions := [Base];
-        uniqId := [fieldVal opcodeField (5'b"01100");
-                   fieldVal funct3Field (3'b"010");
-                   fieldVal funct7Field (7'b"0000000")];
-        inputXform ty pc inst cs1 cs2 ie :=
-          ( LETC in1 <- SignExtend 1 (cs1 @% "val");
-            LETC in2 <- SignExtend 1 (cs2 @% "val");
-            LETC res <- UniBit (TruncMsb Xlen 1) (#in1 + ~#in2 + $1);
-            RetE ((DefSpecOutput ty)
-                    @%[ "wb?" <- $$true ]
-                    @%[ "cdVal" <- ZeroExtendTruncLsb Xlen #res]));
-        outputXform ty (res: SpecOutput @# ty) :=
-          ( RetE (mkIntReg (res @% "cdVal") (res @% "takenPcCap") (res @% "takenPc")));
-        instProperties := {| hasCs1 := true; hasCs2 := true; implicit := 0 |}
-      |};
-      {|instName := "SLTU";
-        xlens := [32; 64];
-        extensions := [Base];
-        uniqId := [fieldVal opcodeField (5'b"01100");
-                   fieldVal funct3Field (3'b"011");
-                   fieldVal funct7Field (7'b"0000000")];
-        inputXform ty pc inst cs1 cs2 ie :=
-          ( LETC in1 <- ZeroExtend 1 (cs1 @% "val");
-            LETC in2 <- ZeroExtend 1 (cs2 @% "val");
-            LETC res <- UniBit (TruncMsb Xlen 1) (#in1 + ~#in2 + $1);
-            RetE ((DefSpecOutput ty)
-                    @%[ "wb?" <- $$true ]
-                    @%[ "cdVal" <- ZeroExtendTruncLsb Xlen #res]));
-        outputXform ty (res: SpecOutput @# ty) :=
-          ( RetE (mkIntReg (res @% "cdVal") (res @% "takenPcCap") (res @% "takenPc")));
-        instProperties := {| hasCs1 := true; hasCs2 := true; implicit := 0 |}
-      |};
-      {|instName := "Xor";
-        xlens := [32; 64];
-        extensions := [Base];
-        uniqId := [fieldVal opcodeField (5'b"01100");
-                   fieldVal funct3Field (3'b"100");
-                   fieldVal funct7Field (7'b"0000000")];
-        inputXform ty pc inst cs1 cs2 ie :=
-          ( RetE ((DefSpecOutput ty)
-                    @%[ "wb?" <- $$true ]
-                    @%[ "cdVal" <- (cs1 @% "val") .^ (cs2 @% "val")]));
-        outputXform ty (res: SpecOutput @# ty) :=
-          ( RetE (mkIntReg (res @% "cdVal") (res @% "takenPcCap") (res @% "takenPc")));
-        instProperties := {| hasCs1 := true; hasCs2 := true; implicit := 0 |}
-      |};
-      {|instName := "Or";
-        xlens := [32; 64];
-        extensions := [Base];
-        uniqId := [fieldVal opcodeField (5'b"01100");
-                   fieldVal funct3Field (3'b"110");
-                   fieldVal funct7Field (7'b"0000000")];
-        inputXform ty pc inst cs1 cs2 ie :=
-          ( RetE ((DefSpecOutput ty)
-                    @%[ "wb?" <- $$true ]
-                    @%[ "cdVal" <- (cs1 @% "val") .| (cs2 @% "val")]));
-        outputXform ty (res: SpecOutput @# ty) :=
-          ( RetE (mkIntReg (res @% "cdVal") (res @% "takenPcCap") (res @% "takenPc")));
-        instProperties := {| hasCs1 := true; hasCs2 := true; implicit := 0 |}
-      |};
-      {|instName := "And";
-        xlens := [32; 64];
-        extensions := [Base];
-        uniqId := [fieldVal opcodeField (5'b"01100");
-                   fieldVal funct3Field (3'b"111");
-                   fieldVal funct7Field (7'b"0000000")];
-        inputXform ty pc inst cs1 cs2 ie :=
-          ( RetE ((DefSpecOutput ty)
-                    @%[ "wb?" <- $$true ]
-                    @%[ "cdVal" <- (cs1 @% "val") .& (cs2 @% "val")]));
-        outputXform ty (res: SpecOutput @# ty) :=
-          ( RetE (mkIntReg (res @% "cdVal") (res @% "takenPcCap") (res @% "takenPc")));
-        instProperties := {| hasCs1 := true; hasCs2 := true; implicit := 0 |}
-      |};
-      {|instName := "SLL";
-        xlens := [32; 64];
-        extensions := [Base];
-        uniqId := [fieldVal opcodeField (5'b"01100");
-                   fieldVal funct3Field (3'b"001");
-                   fieldVal funct7Field (7'b"0000000")];
-        inputXform ty pc inst cs1 cs2 ie :=
-          ( RetE ((DefSpecOutput ty)
-                    @%[ "wb?" <- $$true ]
-                    @%[ "cdVal" <- (cs1 @% "val") <<
-                                     (ZeroExtendTruncLsb (Nat.log2_up Xlen) (cs2 @% "val"))]));
-        outputXform ty (res: SpecOutput @# ty) :=
-          ( RetE (mkIntReg (res @% "cdVal") (res @% "takenPcCap") (res @% "takenPc")));
-        instProperties := {| hasCs1 := true; hasCs2 := true; implicit := 0 |}
-      |};
-      {|instName := "SRL";
-        xlens := [32; 64];
-        extensions := [Base];
-        uniqId := [fieldVal opcodeField (5'b"01100");
-                   fieldVal funct3Field (3'b"101");
-                   fieldVal funct7Field (7'b"0000000")];
-        inputXform ty pc inst cs1 cs2 ie :=
-          ( RetE ((DefSpecOutput ty)
-                    @%[ "wb?" <- $$true ]
-                    @%[ "cdVal" <- UniBit (TruncLsb Xlen 1)
-                                     ((ZeroExtend 1 (cs1 @% "val")) >>>
-                                        (ZeroExtendTruncLsb (Nat.log2_up Xlen) (cs2 @% "val")))]));
-        outputXform ty (res: SpecOutput @# ty) :=
-          ( RetE (mkIntReg (res @% "cdVal") (res @% "takenPcCap") (res @% "takenPc")));
-        instProperties := {| hasCs1 := true; hasCs2 := true; implicit := 0 |}
-      |};
-      {|instName := "SRA";
-        xlens := [32; 64];
-        extensions := [Base];
-        uniqId := [fieldVal opcodeField (5'b"01100");
-                   fieldVal funct3Field (3'b"101");
-                   fieldVal funct7Field (7'b"0100000")];
-        inputXform ty pc inst cs1 cs2 ie :=
-          ( RetE ((DefSpecOutput ty)
-                    @%[ "wb?" <- $$true ]
-                    @%[ "cdVal" <- UniBit (TruncLsb Xlen 1)
-                                     ((SignExtend 1 (cs1 @% "val")) >>>
-                                        (ZeroExtendTruncLsb (Nat.log2_up Xlen) (cs2 @% "val")))]));
-        outputXform ty (res: SpecOutput @# ty) :=
-          ( RetE (mkIntReg (res @% "cdVal") (res @% "takenPcCap") (res @% "takenPc")));
-        instProperties := {| hasCs1 := true; hasCs2 := true; implicit := 0 |}
-      |};
-      {|instName := "AddIW";
-        xlens := [64];
-        extensions := [Base];
-        uniqId := [fieldVal opcodeField (5'b"00110");
-                   fieldVal funct3Field (3'b"000")];
-        inputXform ty pc inst cs1 cs2 ie :=
-          ( RetE ((DefSpecOutput ty)
-                    @%[ "wb?" <- $$true ]
-                    @%[ "cdVal" <- Trunc32Signed Xlen ((cs1 @% "val") + SignExtendTruncLsb Xlen (imm inst))]));
-        outputXform ty (res: SpecOutput @# ty) :=
-          ( RetE (mkIntReg (res @% "cdVal") (res @% "takenPcCap") (res @% "takenPc")));
-        instProperties := {| hasCs1 := true; hasCs2 := false; implicit := 0 |}
-      |};
-      {|instName := "SLLIW";
-        xlens := [64];
-        extensions := [Base];
-        uniqId := [fieldVal opcodeField (5'b"00110");
-                   fieldVal funct3Field (3'b"001");
-                   fieldVal funct7Field (7'b"0000000")];
-        inputXform ty pc inst cs1 cs2 ie :=
-          ( RetE ((DefSpecOutput ty)
-                    @%[ "wb?" <- $$true ]
-                    @%[ "cdVal" <- Trunc32Signed Xlen ((cs1 @% "val") <<
-                                                   (ZeroExtendTruncLsb (Nat.log2_up Xlen) (imm inst)))]));
-        outputXform ty (res: SpecOutput @# ty) :=
-          ( RetE (mkIntReg (res @% "cdVal") (res @% "takenPcCap") (res @% "takenPc")));
-        instProperties := {| hasCs1 := true; hasCs2 := false; implicit := 0 |}
-      |};
-      {|instName := "SRLIW";
-        xlens := [64];
-        extensions := [Base];
-        uniqId := [fieldVal opcodeField (5'b"00110");
-                   fieldVal funct3Field (3'b"101");
-                   fieldVal funct7Field (7'b"0000000")];
-        inputXform ty pc inst cs1 cs2 ie :=
-          ( RetE ((DefSpecOutput ty)
-                    @%[ "wb?" <- $$true ]
-                    @%[ "cdVal" <- (Trunc32Unsigned Xlen (cs1 @% "val")) >>>
-                                     (ZeroExtendTruncLsb (Nat.log2_up Xlen) (imm inst))]));
-        outputXform ty (res: SpecOutput @# ty) :=
-          ( RetE (mkIntReg (res @% "cdVal") (res @% "takenPcCap") (res @% "takenPc")));
-        instProperties := {| hasCs1 := true; hasCs2 := false; implicit := 0 |}
-      |};
-      {|instName := "SRAIW";
-        xlens := [64];
-        extensions := [Base];
-        uniqId := [fieldVal opcodeField (5'b"00110");
-                   fieldVal funct3Field (3'b"101");
-                   fieldVal funct7Field (7'b"0100000")];
-        inputXform ty pc inst cs1 cs2 ie :=
-          ( RetE ((DefSpecOutput ty)
-                    @%[ "wb?" <- $$true ]
-                    @%[ "cdVal" <- (Trunc32Signed Xlen (cs1 @% "val")) >>>
-                                     (ZeroExtendTruncLsb (Nat.log2_up Xlen) (imm inst))]));
-        outputXform ty (res: SpecOutput @# ty) :=
-          ( RetE (mkIntReg (res @% "cdVal") (res @% "takenPcCap") (res @% "takenPc")));
-        instProperties := {| hasCs1 := true; hasCs2 := false; implicit := 0 |}
-      |};
-      {|instName := "AddW";
-        xlens := [64];
-        extensions := [Base];
-        uniqId := [fieldVal opcodeField (5'b"01110");
-                   fieldVal funct3Field (3'b"000");
-                   fieldVal funct7Field (7'b"0000000")];
-        inputXform ty pc inst cs1 cs2 ie :=
-          ( RetE ((DefSpecOutput ty)
-                    @%[ "wb?" <- $$true ]
-                    @%[ "cdVal" <- Trunc32Signed Xlen ((cs1 @% "val") + (cs2 @% "val"))]));
-        outputXform ty (res: SpecOutput @# ty) :=
-          ( RetE (mkIntReg (res @% "cdVal") (res @% "takenPcCap") (res @% "takenPc")));
-        instProperties := {| hasCs1 := true; hasCs2 := false; implicit := 0 |}
-      |};
-      {|instName := "SubW";
-        xlens := [64];
-        extensions := [Base];
-        uniqId := [fieldVal opcodeField (5'b"01110");
-                   fieldVal funct3Field (3'b"000");
-                   fieldVal funct7Field (7'b"0100000")];
-        inputXform ty pc inst cs1 cs2 ie :=
-          ( RetE ((DefSpecOutput ty)
-                    @%[ "wb?" <- $$true ]
-                    @%[ "cdVal" <- Trunc32Signed Xlen (Sub (cs1 @% "val") (cs2 @% "val"))]));
-        outputXform ty (res: SpecOutput @# ty) :=
-          ( RetE (mkIntReg (res @% "cdVal") (res @% "takenPcCap") (res @% "takenPc")));
-        instProperties := {| hasCs1 := true; hasCs2 := false; implicit := 0 |}
-      |};
-      {|instName := "SLLW";
-        xlens := [64];
-        extensions := [Base];
-        uniqId := [fieldVal opcodeField (5'b"01110");
-                   fieldVal funct3Field (3'b"001");
-                   fieldVal funct7Field (7'b"0000000")];
-        inputXform ty pc inst cs1 cs2 ie :=
-          ( RetE ((DefSpecOutput ty)
-                    @%[ "wb?" <- $$true ]
-                    @%[ "cdVal" <- Trunc32Signed Xlen
-                                     ((cs1 @% "val") <<
-                                        (ZeroExtendTruncLsb (Nat.log2_up Xlen) (cs2 @% "val")))]));
-        outputXform ty (res: SpecOutput @# ty) :=
-          ( RetE (mkIntReg (res @% "cdVal") (res @% "takenPcCap") (res @% "takenPc")));
-        instProperties := {| hasCs1 := true; hasCs2 := false; implicit := 0 |}
-      |};
-      {|instName := "SRLW";
-        xlens := [64];
-        extensions := [Base];
-        uniqId := [fieldVal opcodeField (5'b"01110");
-                   fieldVal funct3Field (3'b"101");
-                   fieldVal funct7Field (7'b"0000000")];
-        inputXform ty pc inst cs1 cs2 ie :=
-          ( RetE ((DefSpecOutput ty)
-                    @%[ "wb?" <- $$true ]
-                    @%[ "cdVal" <- (Trunc32Unsigned Xlen (cs1 @% "val")) >>>
-                                     (ZeroExtendTruncLsb (Nat.log2_up Xlen) (cs2 @% "val"))]));
-        outputXform ty (res: SpecOutput @# ty) :=
-          ( RetE (mkIntReg (res @% "cdVal") (res @% "takenPcCap") (res @% "takenPc")));
-        instProperties := {| hasCs1 := true; hasCs2 := false; implicit := 0 |}
-      |};
-      {|instName := "SRAW";
-        xlens := [64];
-        extensions := [Base];
-        uniqId := [fieldVal opcodeField (5'b"01110");
-                   fieldVal funct3Field (3'b"101");
-                   fieldVal funct7Field (7'b"0100000")];
-        inputXform ty pc inst cs1 cs2 ie :=
-          ( RetE ((DefSpecOutput ty)
-                    @%[ "wb?" <- $$true ]
-                    @%[ "cdVal" <- (Trunc32Signed Xlen (cs1 @% "val")) >>>
-                                     (ZeroExtendTruncLsb (Nat.log2_up Xlen) (cs2 @% "val"))]));
-        outputXform ty (res: SpecOutput @# ty) :=
-          ( RetE (mkIntReg (res @% "cdVal") (res @% "takenPcCap") (res @% "takenPc")));
-        instProperties := {| hasCs1 := true; hasCs2 := false; implicit := 0 |}
-      |}
-    ].
-End InstSpec.
+      |}.
+
+  Definition branchInsts: InstEntryFull BaseOutput :=
+    {|xlens := [32; 64];
+      extension := Base;
+      instEntries := [
+        mkBranchInst "BEq" ('b"000") (fun ty rs1 rs2 => RetE (rs1 == rs2));
+        mkBranchInst "BNE" ('b"001") (fun ty rs1 rs2 => RetE !(rs1 == rs2));
+        mkBranchInst "BLT" ('b"100") (fun ty rs1 rs2 =>
+                                        ( LETC a <- SignExtend 1 rs1;
+                                          LETC b <- SignExtend 1 rs2;
+                                          LETC res <- Sub #a #b;
+                                          RetE (unpack Bool (UniBit (TruncMsb Xlen 1) #res))));
+        mkBranchInst "BGE" ('b"101") (fun ty rs1 rs2 =>
+                                        ( LETC a <- SignExtend 1 rs1;
+                                          LETC b <- SignExtend 1 rs2;
+                                          LETC res <- Sub #a #b;
+                                          RetE !(unpack Bool (UniBit (TruncMsb Xlen 1) #res))));
+        mkBranchInst "BLTU" ('b"110") (fun ty rs1 rs2 =>
+                                         ( LETC a <- ZeroExtend 1 rs1;
+                                           LETC b <- ZeroExtend 1 rs2;
+                                           LETC res <- Sub #a #b;
+                                           RetE (unpack Bool (UniBit (TruncMsb Xlen 1) #res))));
+        mkBranchInst "BGEU" ('b"111") (fun ty rs1 rs2 =>
+                                         ( LETC a <- ZeroExtend 1 rs1;
+                                           LETC b <- ZeroExtend 1 rs2;
+                                           LETC res <- Sub #a #b;
+                                           RetE !(unpack Bool (UniBit (TruncMsb Xlen 1) #res))))
+      ]
+    |}.
+
+  Definition mkLdInst (name: string) funct3Val (size: nat) (isCap sign: bool) :=
+    {|instName := name;
+      uniqId := [fieldVal opcodeField (5'b"00000");
+                 fieldVal funct3Field funct3Val];
+      inputXform ty pc inst cs1 cs2 ie :=
+        ( LETC newAddr <- (cs1 @% "val") + SignExtendTruncLsb Xlen (imm inst);
+          LETE baseTop <- getCapBaseTop capAccessors (cs1 @% "cap") (cs1 @% "val");
+          LETC baseBound <- #newAddr >= (#baseTop @% "base");
+          LETC topBound <- ZeroExtend 1 #newAddr + $size <= (#baseTop @% "top");
+          LETE perms <- getCapPerms capAccessors (cs1 @% "cap");
+          LETC fullException
+            : Maybe Data <-
+                (IF !(cs1 @% "tag")
+                 then Valid (Const ty (natToWord Xlen CapTagViolation))
+                 else (IF isSealed capAccessors (cs1 @% "cap")
+                       then Valid (Const ty (natToWord Xlen CapSealViolation))
+                       else (IF !(#perms @% "LD")
+                             then Valid (Const ty (natToWord Xlen CapLdViolation))
+                             else (IF !(#baseBound && #topBound)
+                                   then Valid (Const ty (natToWord Xlen CapBoundsViolation))
+                                   else StaticIf isCap
+                                          (isNotZero (ZeroExtendTruncLsb (Nat.log2_up ((Xlen + CapSz)/8)) #newAddr))
+                                          (Valid (Const ty (natToWord Xlen CapLdMisaligned)))
+                                          Invalid))));
+          RetE ((DefBaseOutput ty)
+                  @%[ "exception?" <- #fullException @% "valid" ]
+                  @%[ "exceptionCause" <- #fullException @% "data" ]
+                  @%[ "pcMemAddr" <- #newAddr ]
+                  @%[ "memCap?" <- $$isCap ]
+                  @%[ "memSize" <- Const ty (natToWord MemSizeSz size) ]
+                  @%[ "mem?" <- $$true ]
+                  @%[ "ldSigned?" <- $$sign ]
+                  @%[ "ldPerms" <- #perms ]));
+      instProperties := {| hasCs1 := true; hasCs2 := false; implicit := 0 |}
+    |}.
+
+  Definition ldInsts: InstEntryFull BaseOutput :=
+    {|xlens := [32; 64];
+      extension := Base;
+      instEntries := [
+        mkLdInst "CLB"  ('b"000") 1 false true;
+        mkLdInst "CLH"  ('b"001") 2 false true;
+        mkLdInst "CLW"  ('b"010") 4 false true;
+        mkLdInst "CLBU" ('b"100") 1 false false;
+        mkLdInst "CLHU" ('b"101") 2 false false
+      ]
+    |}.
+  
+  Definition ld32Insts: InstEntryFull BaseOutput :=
+    {|xlens := [32];
+      extension := Base;
+      instEntries := [
+        mkLdInst "CLC"  ('b"011") 8 true  false
+      ]
+    |}.
+  
+  Definition ld64Insts: InstEntryFull BaseOutput :=
+    {|xlens := [64];
+      extension := Base;
+      instEntries := [
+        mkLdInst "CLWU" ('b"110") 4 false false
+      ]
+    |}.
+
+  Definition mkStInst (name: string) funct3Val (size: nat) (isCap: bool) :=
+    {|instName := name;
+      uniqId := [fieldVal opcodeField (5'b"01000");
+                 fieldVal funct3Field funct3Val];
+      inputXform ty pc inst cs1 cs2 ie :=
+        ( LETC newAddr <- (cs1 @% "val") + SignExtendTruncLsb Xlen (imm inst);
+          LETE baseTop <- getCapBaseTop capAccessors (cs1 @% "cap") (cs1 @% "val");
+          LETC baseBound <- #newAddr >= (#baseTop @% "base");
+          LETC topBound <- ZeroExtend 1 #newAddr + $size <= (#baseTop @% "top");
+          LETE perms <- getCapPerms capAccessors (cs1 @% "cap");
+          LETE perms2 <- getCapPerms capAccessors (cs2 @% "cap");
+          LETC fullException
+            : Maybe Data <-
+                (IF !(cs1 @% "tag")
+                 then Valid (Const ty (natToWord Xlen CapTagViolation))
+                 else (IF isSealed capAccessors (cs1 @% "cap")
+                       then Valid (Const ty (natToWord Xlen CapSealViolation))
+                       else (IF !(#perms @% "SD")
+                             then Valid (Const ty (natToWord Xlen CapStViolation))
+                             else (IF !(#perms @% "SL") && (cs2 @% "tag") && !(#perms2 @% "GL")
+                                   then Valid (Const ty (natToWord Xlen CapStLocalViolation))
+                                   else (IF !(#baseBound && #topBound)
+                                         then Valid (Const ty (natToWord Xlen CapBoundsViolation))
+                                         else StaticIf isCap
+                                                (isNotZero (ZeroExtendTruncLsb (Nat.log2_up ((Xlen + CapSz)/8)) #newAddr))
+                                                (Valid (Const ty (natToWord Xlen CapStMisaligned)))
+                                                Invalid)))));
+          RetE ((DefBaseOutput ty)
+                  @%[ "exception?" <- #fullException @% "valid" ]
+                  @%[ "exceptionCause" <- #fullException @% "data" ]
+                  @%[ "pcMemAddr" <- #newAddr ]
+                  @%[ "memCap?" <- $$isCap ]
+                  @%[ "memSize" <- Const ty (natToWord MemSizeSz size) ]
+                  @%[ "mem?" <- $$true ]
+                  @%[ "store?" <- $$true ]
+                  @%[ "cdTag" <- cs2 @% "tag"]
+                  @%[ "cdCap" <- cs2 @% "cap"]
+                  @%[ "cdVal" <- cs2 @% "val"] ));
+      instProperties := {| hasCs1 := true; hasCs2 := true; implicit := 0 |}
+    |}.
+
+  Definition stInsts: InstEntryFull BaseOutput :=
+    {|xlens := [32; 64];
+      extension := Base;
+      instEntries := [
+        mkStInst "CSB"  ('b"000") 1 false;
+        mkStInst "CSH"  ('b"001") 2 false;
+        mkStInst "CSW"  ('b"010") 4 false
+      ]
+    |}.
+  
+  Definition st32Insts: InstEntryFull BaseOutput :=
+    {|xlens := [32];
+      extension := Base;
+      instEntries := [
+        mkStInst "CSC"  ('b"011") 8 true
+      ]
+    |}.
+  
+  Definition st64Insts: InstEntryFull BaseOutput :=
+    {|xlens := [64];
+      extension := Base;
+      instEntries := [
+      ]
+    |}.
+
+  Definition jumpInsts: InstEntryFull BaseOutput :=
+    {|xlens := [32; 64];
+      extension := Base;
+      instEntries := [
+        {|instName := "CJAL";
+          uniqId := [fieldVal opcodeField (truncMsb (7'h"6f"))];
+          inputXform ty pc inst cs1 cs2 ie :=
+            ( LETC newAddr <- (pc @% "val") + SignExtendTruncLsb Xlen (jalOffset inst);
+              LETC linkAddr <- (pc @% "val") + ITE (isInstNotCompressed inst) $4 $2;
+              RetE ((DefBaseOutput ty)
+                      @%[ "wb?" <- $$true ]
+                      @%[ "cdTag" <- $$true ]
+                      @%[ "cdCap" <- seal capAccessors (pc @% "cap") (getOTypeFromIe capAccessors ie) ]
+                      @%[ "cdVal" <- #linkAddr ]
+                      @%[ "mayChangePc?" <- $$true ]
+                      @%[ "taken?" <- $$true ]
+                      @%[ "pcMemAddr" <- #newAddr ]
+                      @%[ "exception?" <- if compressed
+                                          then $$false
+                                          else isNotZero (ZeroExtendTruncLsb 2 #newAddr) ]
+                      @%[ "exceptionCause" <- if compressed
+                                              then Const ty (natToWord Xlen 0)
+                                              else $InstMisaligned ]
+                      @%[ "exceptionCausePc?" <- $$true ]));
+          instProperties := {| hasCs1 := false; hasCs2 := false; implicit := 0 |}
+        |};
+        {|instName := "CJALR";
+          uniqId := [fieldVal opcodeField (truncMsb (7'h"67"));
+                     fieldVal funct3Field (3'h"0")];
+          inputXform ty pc inst cs1 cs2 ie :=
+            ( LETC newAddrTemp <- (cs1 @% "val") + SignExtendTruncLsb Xlen (imm inst);
+              LETC newAddr <- ZeroExtendTruncLsb Xlen ({< ZeroExtendTruncMsb (Xlen - 1) #newAddrTemp, $$WO~0 >});
+              LETC linkAddr <- (pc @% "val") + ITE (isInstNotCompressed inst) $4 $2;
+              LETE perms <- getCapPerms capAccessors (cs1 @% "cap");
+              LETC fullException
+                : Pair (Maybe Data) Bool <-
+                    (IF !(cs1 @% "tag")
+                     then mkPair (Valid (Const ty (natToWord Xlen CapTagViolation))) ($$false)
+                     else (IF isSealed capAccessors (cs1 @% "cap") &&
+                             (!isSentry capAccessors (cs1 @% "cap") || isNotZero (imm inst) )
+                           then mkPair (Valid (Const ty (natToWord Xlen CapSealViolation))) ($$false)
+                           else (IF !(#perms @% "EX")
+                                 then mkPair (Valid (Const ty (natToWord Xlen CapExecViolation))) ($$false)
+                                 else if compressed
+                                      then mkPair Invalid ($$false)
+                                      else mkPair (Valid (Const ty (natToWord Xlen InstMisaligned))) ($$true))));
+              LETC ieSentry <- isIeSentry capAccessors (cs1 @% "cap");
+              LETC idSentry <- isIdSentry capAccessors (cs1 @% "cap");
+              RetE ((DefBaseOutput ty)
+                      @%[ "wb?" <- $$true ]
+                      @%[ "cdTag" <- $$true ]
+                      @%[ "cdCap" <- seal capAccessors (pc @% "cap") (getOTypeFromIe capAccessors ie) ]
+                      @%[ "cdVal" <- #linkAddr ]
+                      @%[ "mayChangePc?" <- $$true ]
+                      @%[ "taken?" <- $$true ]
+                      @%[ "pcMemAddr" <- #newAddr ]
+                      @%[ "changePcCap?" <- $$true ]
+                      @%[ "pcCap" <- unseal capAccessors (cs1 @% "cap") ]
+                      @%[ "exception?" <- #fullException @% "fst" @% "valid" ]
+                      @%[ "exceptionCause" <- #fullException @% "fst" @% "data" ]
+                      @%[ "exceptionCausePc?" <- #fullException @% "snd" ]
+                      @%[ "changeIe?" <- #ieSentry || #idSentry ]
+                      @%[ "newIe" <- #ieSentry ] ));
+          instProperties := {| hasCs1 := true; hasCs2 := false; implicit := 0 |}
+        |}
+      ]
+    |}.
+
+  Definition interruptInsts: InstEntryFull BaseOutput :=
+    {|xlens := [32; 64];
+      extension := Base;
+      instEntries := [
+        {|instName := "FenceI";
+          uniqId := [fieldVal opcodeField (5'b"00011");
+                     fieldVal funct3Field (3'b"001")];
+          inputXform ty pc inst cs1 cs2 ie :=
+            ( RetE ((DefBaseOutput ty)
+                      @%[ "interrupt?" <- $$true ]
+                      @%[ "exceptionCause" <- Const ty (natToWord Xlen FenceI) ]));
+          instProperties := {| hasCs1 := false; hasCs2 := false; implicit := 0 |}
+        |};
+        {|instName := "WFI";
+          uniqId := [fieldVal opcodeField (5'b"11100");
+                     fieldVal rdFixedField (5'b"00000");
+                     fieldVal funct3Field (3'b"000");
+                     fieldVal rs1FixedField (5'b"00000");
+                     fieldVal rs2FixedField (5'b"00101");
+                     fieldVal funct7Field (7'b"0001000")];
+          inputXform ty pc inst cs1 cs2 ie :=
+            ( RetE ((DefBaseOutput ty)
+                      @%[ "interrupt?" <- $$true ]
+                      @%[ "exceptionCause" <- Const ty (natToWord Xlen WFI) ]));
+          instProperties := {| hasCs1 := false; hasCs2 := false; implicit := 0 |}
+        |}
+      ]
+    |}.
+
+  Definition specBaseFuncUnit : FuncEntry :=
+    {|localFuncInput := BaseOutput;
+      localFuncOutput := BaseOutput;
+      localFunc ty x := RetE x;
+      outputXform := baseOutputXform;
+      insts := [aluInsts; alu64Insts; capInsts; branchInsts; ldInsts; ld32Insts; ld64Insts; stInsts; st32Insts; st64Insts; jumpInsts; interruptInsts]
+    |}.
+
+  Definition specBaseInsts : list (InstEntry BaseOutput) := filtInsts (mkFiltFuncEntry specBaseFuncUnit).
+
+  Ltac simplify_field field :=
+    repeat match goal with
+           | |- context [field ?P] =>
+               let sth := fresh "sth" in
+               let Heq_sth := fresh "Heq_sth" in
+               remember (field P) as sth eqn: Heq_sth; simpl in Heq_sth; rewrite Heq_sth; clear Heq_sth sth
+           end.
+
+  Theorem uniqAluIds: NoDup (map (@uniqId _ BaseOutput) specBaseInsts).
+  Proof.
+    unfold specBaseInsts, mkFiltFuncEntry, filtInsts, specBaseFuncUnit, insts, localFuncInput, localFuncOutput, fold_left.
+    pose proof extsHasBase as base.
+    simplify_field (@extension procParams BaseOutput).
+    destruct (in_dec Extension_eq_dec Base supportedExts); [| unfold getBool; rewrite ?andb_false_r; simpl; auto; constructor].
+    simplify_field (@xlens procParams BaseOutput).
+    destruct (xlenIs32_or_64) as [H | H]; do 2 (rewrite H; simpl);
+      repeat constructor; unfold In, not; intros;
+      repeat match goal with
+        | H: ?p \/ ?q |- _ => destruct H; try discriminate
+        end; auto.
+  Qed.
+
+End InstBaseSpec.
